pk_auth/client_proofs.v
@@ -22,10 +22,10 @@ Variable N : namespace.
 
 Context `{!PK}.
 
-Lemma public_msg1I n kI kR nI :
+Lemma public_msg1I kI kR nI :
   let sI := mk_key_share nI in
   pk_auth_ctx N -∗
-  session_weak' N kI kR nI n -∗
+  session_weak' N kI kR nI -∗
   minted nI -∗
   □ is_priv_key nI kI kR -∗
   public (TKey Seal kI) -∗
@@ -38,7 +38,7 @@ iPoseProof (mk_key_share_secret_of with "s_nI p_nI") as "p_sI".
 iApply public_TSealIS; eauto.
 - iModIntro. iExists (mk_key_share nI), kI. do !iSplit => //.
   + iIntros "!> #?". iApply "p_sI". by eauto.
-  + iRight. by iExists n, nI; eauto.
+  + iRight. by iExists nI; eauto.
 - rewrite minted_of_list /= mk_key_share_minted. by eauto.
 iIntros "!> #p_dkR". rewrite public_of_list /=. do !iSplit => //.
 iApply "p_sI". iModIntro. by iRight.
@@ -68,27 +68,25 @@ iPoseProof (public_TSealE with "p_m2 m2P") as "{p_m2} [p_m2 | p_m2]".
   do !iSplit => //.
 Qed.
 
-Lemma init_finish dq n kI kR nI sR :
+Lemma init_finish kI kR nI sR :
   let sI := mk_key_share nI in
   let kS := mk_session_key Init nI sR in
   pk_auth_ctx N -∗
-  ●Ph{dq} n -∗
-  session_weak' N kI kR nI n -∗
+  session_weak' N kI kR nI -∗
   minted nI -∗
   □ is_priv_key nI kI kR -∗
   secret_of sR kI kR -∗
   resp_accepted N kI kR sI sR -∗
   term_token nI (⊤ ∖ ↑N.@"success") -∗
   init_confirm kI kR ={⊤}=∗
-  ▷ (●Ph{dq} n ∗
-     □ confirmation Init kI kR kS ∗
-     session_weak N Init kI kR kS n ∗
+  ▷ (□ confirmation Init kI kR kS ∗
+     session_weak N Init kI kR kS ∗
      init_finished N kR sR ∗
      (corruption kI kR ∨
       session_key_meta_token N kI kR kS (↑N.@"init") ∗
-      session_key N kI kR kS n)).
+      session_key N kI kR kS)).
 Proof.
-iIntros "%sI %kS (#ctx & _) hon #sess #s_nI #p_nI #p_sR #accepted token confirm".
+iIntros "%sI %kS (#ctx & _) #sess #s_nI #p_nI #p_sR #accepted token confirm".
 iMod ("confirm" $! nI sR) as "#confirm".
 iAssert (secret_of sI kI kR) as "p_sI".
   by iApply mk_key_share_secret_of.
@@ -106,15 +104,11 @@ iDestruct "accepted" as "[fail|accepted]".
   iSplit; eauto.
   iLeft. iApply "p_sR". by iApply "p_sI".
 iDestruct "accepted"
-  as "(%n' & %n'' & %nI' & %nR & %n''n' &
+  as "(%nI' & %nR &
        #sess' & #sess'' &
        %e_sI & -> & #p_nR & #accepted & confirmed)".
 move/mk_key_share_inj: e_sI => <-.
-iDestruct (session_weak'_agree with "sess' sess") as "(_ & _ & ->)".
-iAssert (⌜n' = n⌝)%I as "#->".
-  iDestruct "sess''" as "[hon' _]".
-  iPoseProof (phase_auth_frag_agree with "hon hon'") as "%n'n".
-  iPureIntro; lia.
+iDestruct (session_weak'_agree with "sess' sess") as "(_ & _)".
 iMod (session_begin _ Init nI nR (kI, kR) with "ctx [resp_token] token_sess")
   as "[#sessI _]".
 - solve_ndisj.
@@ -122,7 +116,7 @@ iMod (session_begin _ Init nI nR (kI, kR) with "ctx [resp_token] token_sess")
 iModIntro. iModIntro. iFrame. iSplit; eauto. iSplitR.
   by iExists _, _; eauto.
 iSplitR.
-  iRight. iExists nI, nR, kI, n. do !iSplit => //; by eauto.
+  iRight. iExists nI, nR, kI. do !iSplit => //; by eauto.
 iRight. iSplitL.
   iExists nI, nR; by eauto.
 iExists nI, nR; do !iSplit => //; eauto.
@@ -144,38 +138,34 @@ Qed.
 Ltac protocol_failure :=
   by intros; wp_pures; iApply ("Hpost" $! None); iFrame.
 
-Lemma wp_pk_auth_init c kI kR dq n T :
+Lemma wp_pk_auth_init c kI kR :
   channel c -∗
   cryptis_ctx -∗
   pk_auth_ctx N -∗
   public (TKey Seal kI) -∗
   public (TKey Seal kR) -∗
-  honest n T -∗
-  {{{ init_confirm kI kR ∗ ●Ph{dq} n }}}
+  {{{ init_confirm kI kR }}}
     pk_auth_init N c mk_key_share_impl (mk_session_key_impl Init)
     kI (TKey Seal kR)
   {{{ okS, RET (repr okS);
-      ●Ph{dq} n ∗
       if okS is Some kS then
         minted kS ∗
         □ confirmation Init kI kR kS ∗
-        session_weak N Init kI kR kS n ∗
-        if in_honest kI kR T then
+        session_weak N Init kI kR kS ∗
+        (corruption kI kR ∨
           session_key_meta_token N kI kR kS (↑N.@"init") ∗
-          session_key N kI kR kS n
-        else True
+          session_key N kI kR kS)
       else True }}}.
 Proof.
-rewrite /pk_auth_init /in_honest bool_decide_decide.
-iIntros "#chan_c #ctx #ctx' #p_kI #p_kR #hon %Ψ !> [confirm phase] Hpost".
+rewrite /pk_auth_init.
+iIntros "#chan_c #ctx #ctx' #p_kI #p_kR %Ψ !> confirm Hpost".
 wp_pures. wp_apply wp_pkey. wp_pures.
 wp_bind (mk_key_share_impl _).
 iApply (wp_mk_key_share kI kR) => //.
 iIntros "!> %nI (#s_nI & #p_nI & token)".
 rewrite (term_token_difference _ (↑N.@"success")); eauto.
 iDestruct "token" as "[token_succ token]".
-iMod (session_weak'_set N kI kR _ _ with "[#] token_succ") as "#sess".
-  by iApply phase_auth_frag.
+iMod (session_weak'_set N kI kR _ with "token_succ") as "#sess".
 wp_pures.
 iPoseProof (mk_key_share_secret_of with "s_nI p_nI") as "p_sI".
 wp_list. wp_term_of_list. wp_apply wp_aenc. wp_pures.
@@ -190,22 +180,12 @@ wp_eq_term e; last protocol_failure; subst pkR'.
 iPoseProof (public_msg2E with "[//] [//] [//]")
   as "{p_m2} (s_sR & p_sR & accepted)".
 wp_pures.
-iMod (init_finish with "ctx' phase sess s_nI p_nI p_sR accepted token confirm")
-  as "(phase & #confirmed & #sess_weak & #finished & session)"; eauto.
+iMod (init_finish with "ctx' sess s_nI p_nI p_sR accepted token confirm")
+  as "(#confirmed & #sess_weak & #finished & session)"; eauto.
 wp_bind (mk_session_key_impl _ _ _). iApply wp_mk_session_key => //.
 iIntros "!> _". wp_pures. wp_apply wp_aenc. wp_pures. wp_bind (send _ _).
 iApply wp_send => //.
   by iApply public_msg3I.
-case: decide => [[kIP kRP]|_]; last first.
-  wp_pures. iApply ("Hpost" $! (Some (mk_session_key Init nI sR))).
-  iFrame. iModIntro. iSplit; eauto. by iApply mk_session_key_minted.
-iDestruct "session" as "[[#fail|#fail]|session]".
-- iPoseProof (secret_atI _ kIP with "hon") as "sec".
-  iMod (honest_public with "ctx sec phase fail") as "#contra" => //.
-  wp_pures. iDestruct "contra" as "[]".
-- iPoseProof (secret_atI _ kRP with "hon") as "sec".
-  iMod (honest_public with "ctx sec phase fail") as "#contra" => //.
-  wp_pures. iDestruct "contra" as "[]".
 wp_pures. iApply ("Hpost" $! (Some (mk_session_key Init nI sR))).
 iFrame. iModIntro. iSplit; eauto. by iApply mk_session_key_minted.
 Qed.
