pk_auth/server_proofs.v
@@ -43,32 +43,29 @@ iPoseProof (public_TSealE with "p_m1 m1P") as "{p_m1} [p_m1 | p_m1]".
   do !iSplit => //.
 Qed.
 
-Lemma resp_accept dq n E kI kR sI nR :
+Lemma resp_accept E kI kR sI nR :
   ↑N ⊆ E →
   let kS := mk_session_key Resp nR sI in
   term_token nR ⊤ -∗
   resp_confirm kR -∗
   pk_auth_ctx N -∗
-  ●Ph{dq} n -∗
   □ is_priv_key nR kI kR -∗
   init_started N kI kR sI ={E}=∗
-  ●Ph{dq} n ∗
   □ confirmation Resp kI kR kS ∗
-  session_weak' N kI kR nR n ∗
-  session_weak N Resp kI kR kS n ∗
+  session_weak' N kI kR nR ∗
+  session_weak N Resp kI kR kS ∗
   resp_waiting N kI kR sI nR ∗
   resp_accepted N kI kR sI (mk_key_share nR).
 Proof.
-iIntros (?) "%kS token conf (#ctx & _) hon #p_nR #started".
+iIntros (?) "%kS token conf (#ctx & _) #p_nR #started".
 iMod ("conf" $! kI sI nR) as "#conf".
 rewrite (term_token_difference _ (↑N.@"session")) //.
 iDestruct "token" as "[token_sess token]".
 rewrite (term_token_difference _ (↑N.@"success") (_ ∖ _)) //; last first.
   solve_ndisj.
 iDestruct "token" as "[token_succ _]".
-iMod (session_weak'_set N kI kR nR n with "[#] token_succ") as "#sess".
-  by iApply phase_auth_frag.
-iDestruct "started" as "[#fail|(%n' & %nI & -> & #sess' & #p_nI)]".
+iMod (session_weak'_set N kI kR nR with "token_succ") as "#sess".
+iDestruct "started" as "[#fail|(%nI & -> & #sess' & #p_nI)]".
   iModIntro. iFrame. iSplit; eauto. iSplit => //. iSplit.
     by iExists _, _; eauto.
   iSplitL; iLeft => //.
@@ -78,16 +75,12 @@ iMod (session_begin _ Resp nI nR (kI, kR)
        with "ctx [] token_sess") as "[#sessR waiting]".
 - solve_ndisj.
 - rewrite /=. by eauto.
-iAssert (⌜n' ≤ n⌝)%I as "%n'n".
-  iDestruct "sess'" as "[hon' _]".
-  by iApply (phase_auth_frag_agree with "[hon]").
-iPoseProof (phase_auth_frag with "hon") as "#?".
 iFrame. iModIntro. iSplit; eauto. iSplit => //. iSplit.
   rewrite mk_session_keyC in @kS *.
   by iExists _, _; eauto.
 iSplitL.
   iRight. iExists nI. by eauto.
-iRight. iExists n, n', nI, nR.
+iRight. iExists nI, nR.
 by do !iSplit => //.
 Qed.
 
@@ -123,25 +116,25 @@ iDestruct (public_TSealE with "p_m3 [//]") as "{p_m3} [p_m3|p_m3]".
 - by iDestruct "p_m3" as "(#p_m3 & _)".
 Qed.
 
-Lemma resp_finish E kI kR sI nR n :
+Lemma resp_finish E kI kR sI nR :
   let sR := mk_key_share nR in
   let kS := mk_session_key Resp nR sI in
   ↑N ⊆ E →
   pk_auth_ctx N -∗
-  session_weak' N kI kR nR n -∗
+  session_weak' N kI kR nR -∗
   minted nR -∗
   □ is_priv_key nR kI kR -∗
   init_finished N kR sR -∗
   resp_waiting N kI kR sI nR ={E}=∗
   ▷ (corruption kI kR ∨
      session_key_meta_token N kI kR kS (↑N.@"resp") ∗
-     session_key N kI kR kS n).
+     session_key N kI kR kS).
 Proof.
 iIntros "%sR %kS % #(ctx & _) #sess #s_nR #p_nR [#fail|#finished] waiting".
   iPoseProof (mk_key_share_secret_of with "s_nR p_nR") as "p_sR".
   iModIntro. iLeft. by iApply "p_sR".
 iDestruct "finished"
-  as "(%nI' & %nR' & %kI' & %n' &
+  as "(%nI' & %nR' & %kI' &
        #sessWI & #sessWR & %e_sR & p_nI & _ & confirmedI & sessI & sessR')".
 move/mk_key_share_inj: e_sR => <- {nR'}.
 iDestruct "waiting" as "[[#fail token]|waiting]".
@@ -150,7 +143,7 @@ iDestruct "waiting" as "(%nI & -> & #sessR & #confirmedR & waiting)".
 move: @kS; rewrite -mk_session_keyC => kS.
 iPoseProof (session_agree with "sessR sessR'") as "{sessR'} %e" => //.
 case: e => <- <-.
-iPoseProof (session_weak'_agree with "sessWR sess") as "(_ & _ & ->)".
+iPoseProof (session_weak'_agree with "sessWR sess") as "(_ & _)".
 iMod ("waiting" with "[] sessI") as "[_ >finished]".
   solve_ndisj.
 rewrite /=.
@@ -162,29 +155,26 @@ Qed.
 Ltac protocol_failure :=
   by intros; wp_pures; iApply ("Hpost" $! None); iFrame.
 
-Lemma wp_pk_auth_resp c kR dq n T :
+Lemma wp_pk_auth_resp c kR :
   channel c -∗
   cryptis_ctx -∗
   pk_auth_ctx N -∗
   public (TKey Seal kR) -∗
-  honest n T -∗
-  {{{ resp_confirm kR ∗ ●Ph{dq} n }}}
+  {{{ resp_confirm kR }}}
     pk_auth_resp N c mk_key_share_impl (mk_session_key_impl Resp) kR
   {{{ res, RET (repr res);
-      ●Ph{dq} n ∗
       if res is Some (pkI, kS) then
          ∃ kI, ⌜pkI = TKey Seal kI⌝ ∗
                public pkI ∗
                minted kS ∗
                □ confirmation Resp kI kR kS ∗
-               session_weak N Resp kI kR kS n ∗
-               if in_honest kI kR T then
+               session_weak N Resp kI kR kS ∗
+               (corruption kI kR ∨
                 session_key_meta_token N kI kR kS (↑N.@"resp") ∗
-                session_key N kI kR kS n
-               else True
+                session_key N kI kR kS)
        else True }}}.
 Proof.
-iIntros "#? #ctx #ctx' #e_kR #hon %Ψ !> [confirm phase] Hpost".
+iIntros "#? #ctx #ctx' #e_kR %Ψ !> confirm Hpost".
 iPoseProof "ctx'" as "(inv & _)".
 rewrite /pk_auth_resp; wp_pures.
 wp_apply wp_pkey. wp_pures.
@@ -201,8 +191,8 @@ iDestruct (public_msg1E with "[] Hm1")
 wp_pures.
 wp_bind (mk_key_share_impl _). iApply (wp_mk_key_share kI kR) => //.
 iIntros "!> %nR (#s_nR & #p_nR & token)".
-iMod (resp_accept with "token confirm [//] phase [//] [//]")
-  as "(phase & #confirmed & #? & #sess_weak & waiting & #accepted)" => //.
+iMod (resp_accept with "token confirm [//] [//] [//]")
+  as "(#confirmed & #? & #sess_weak & waiting & #accepted)" => //.
 wp_pures. wp_list; wp_term_of_list. wp_apply wp_aenc. wp_pures.
 iAssert (secret_of (mk_key_share nR) kI kR) as "p_sR".
   by iApply mk_key_share_secret_of.
@@ -215,30 +205,10 @@ wp_eq_term e; last protocol_failure; subst m3.
 iPoseProof (public_msg3E with "[//] [//] [//]") as "finished".
 wp_pures.
 iMod (resp_finish with "[] [] [] [] [] waiting") as "session" => //.
-case: (decide (TKey Open kI ∈ T ∧ TKey Open kR ∈ T)) => [[kIP kRP]|pub]; last first.
-  wp_bind (mk_session_key_impl _ _ _). iApply wp_mk_session_key => //.
-  iIntros "!> _". wp_pures.
-  iApply ("Hpost" $! (Some (TKey Seal kI, mk_session_key Resp nR sI))).
-  iModIntro. iFrame. iExists kI.
-  rewrite /in_honest bool_decide_decide decide_False //.
-  do 3!iSplit => //; eauto.
-  by iApply mk_session_key_minted => //.
-iDestruct "session" as "[[#fail|#fail]|session]".
-- wp_bind (mk_session_key_impl _ _ _). iApply wp_mk_session_key => //.
-  iIntros "!> _".
-  iPoseProof (secret_atI _ kIP with "hon") as "sec".
-  iMod (honest_public with "ctx sec phase fail") as "contra"; eauto.
-  wp_pures. by iDestruct "contra" as "[]".
-- wp_bind (mk_session_key_impl _ _ _). iApply wp_mk_session_key => //.
-  iIntros "!> _".
-  iPoseProof (secret_atI _ kRP with "hon") as "sec".
-  iMod (honest_public with "ctx sec phase fail") as "contra"; eauto.
-  wp_pures. by iDestruct "contra" as "[]".
 wp_bind (mk_session_key_impl _ _ _). iApply wp_mk_session_key => //.
 iIntros "!> _". wp_pures.
 iApply ("Hpost" $! (Some (TKey Seal kI, mk_session_key Resp nR sI))).
-iModIntro. iFrame. iExists kI.
-rewrite /in_honest bool_decide_decide decide_True //.
+iModIntro. iFrame.
 do 3!iSplit => //; eauto.
 by iApply mk_session_key_minted => //.
 Qed.
